Source/Dafny/Scanner.cs
@@ -211,8 +211,8 @@ public class UTF8Buffer: Buffer {
 public class Scanner {
 	const char EOL = '\n';
 	const int eofSym = 0; /* pdt */
-	const int maxT = 120;
-	const int noSym = 120;
+	const int maxT = 122;
+	const int noSym = 122;
 
 
 	[ContractInvariantMethod]
@@ -509,52 +509,54 @@ public class Scanner {
 			case "yields": t.kind = 34; break;
 			case "returns": t.kind = 35; break;
 			case "method": t.kind = 39; break;
-			case "comethod": t.kind = 40; break;
-			case "constructor": t.kind = 41; break;
-			case "modifies": t.kind = 42; break;
-			case "free": t.kind = 43; break;
-			case "requires": t.kind = 44; break;
-			case "ensures": t.kind = 45; break;
-			case "decreases": t.kind = 46; break;
-			case "reads": t.kind = 47; break;
-			case "yield": t.kind = 48; break;
-			case "bool": t.kind = 49; break;
-			case "nat": t.kind = 50; break;
-			case "int": t.kind = 51; break;
-			case "set": t.kind = 52; break;
-			case "multiset": t.kind = 53; break;
-			case "seq": t.kind = 54; break;
-			case "map": t.kind = 55; break;
-			case "object": t.kind = 56; break;
-			case "function": t.kind = 57; break;
-			case "predicate": t.kind = 58; break;
-			case "copredicate": t.kind = 59; break;
-			case "label": t.kind = 61; break;
-			case "break": t.kind = 62; break;
-			case "where": t.kind = 63; break;
-			case "return": t.kind = 65; break;
-			case "assume": t.kind = 67; break;
-			case "new": t.kind = 68; break;
-			case "if": t.kind = 71; break;
-			case "else": t.kind = 72; break;
-			case "case": t.kind = 73; break;
-			case "while": t.kind = 75; break;
-			case "invariant": t.kind = 76; break;
-			case "match": t.kind = 77; break;
-			case "assert": t.kind = 78; break;
-			case "print": t.kind = 79; break;
-			case "forall": t.kind = 80; break;
-			case "parallel": t.kind = 81; break;
-			case "calc": t.kind = 82; break;
-			case "in": t.kind = 100; break;
-			case "false": t.kind = 107; break;
-			case "true": t.kind = 108; break;
-			case "null": t.kind = 109; break;
-			case "this": t.kind = 110; break;
-			case "fresh": t.kind = 111; break;
-			case "old": t.kind = 112; break;
-			case "then": t.kind = 113; break;
-			case "exists": t.kind = 116; break;
+			case "lemma": t.kind = 40; break;
+			case "comethod": t.kind = 41; break;
+			case "colemma": t.kind = 42; break;
+			case "constructor": t.kind = 43; break;
+			case "modifies": t.kind = 44; break;
+			case "free": t.kind = 45; break;
+			case "requires": t.kind = 46; break;
+			case "ensures": t.kind = 47; break;
+			case "decreases": t.kind = 48; break;
+			case "reads": t.kind = 49; break;
+			case "yield": t.kind = 50; break;
+			case "bool": t.kind = 51; break;
+			case "nat": t.kind = 52; break;
+			case "int": t.kind = 53; break;
+			case "set": t.kind = 54; break;
+			case "multiset": t.kind = 55; break;
+			case "seq": t.kind = 56; break;
+			case "map": t.kind = 57; break;
+			case "object": t.kind = 58; break;
+			case "function": t.kind = 59; break;
+			case "predicate": t.kind = 60; break;
+			case "copredicate": t.kind = 61; break;
+			case "label": t.kind = 63; break;
+			case "break": t.kind = 64; break;
+			case "where": t.kind = 65; break;
+			case "return": t.kind = 67; break;
+			case "assume": t.kind = 69; break;
+			case "new": t.kind = 70; break;
+			case "if": t.kind = 73; break;
+			case "else": t.kind = 74; break;
+			case "case": t.kind = 75; break;
+			case "while": t.kind = 77; break;
+			case "invariant": t.kind = 78; break;
+			case "match": t.kind = 79; break;
+			case "assert": t.kind = 80; break;
+			case "print": t.kind = 81; break;
+			case "forall": t.kind = 82; break;
+			case "parallel": t.kind = 83; break;
+			case "calc": t.kind = 84; break;
+			case "in": t.kind = 102; break;
+			case "false": t.kind = 109; break;
+			case "true": t.kind = 110; break;
+			case "null": t.kind = 111; break;
+			case "this": t.kind = 112; break;
+			case "fresh": t.kind = 113; break;
+			case "old": t.kind = 114; break;
+			case "then": t.kind = 115; break;
+			case "exists": t.kind = 118; break;
 			default: break;
 		}
 	}
@@ -696,68 +698,68 @@ public class Scanner {
 			case 30:
 				{t.kind = 36; break;}
 			case 31:
-				{t.kind = 60; break;}
+				{t.kind = 62; break;}
 			case 32:
-				{t.kind = 64; break;}
-			case 33:
 				{t.kind = 66; break;}
+			case 33:
+				{t.kind = 68; break;}
 			case 34:
-				{t.kind = 69; break;}
+				{t.kind = 71; break;}
 			case 35:
-				{t.kind = 70; break;}
+				{t.kind = 72; break;}
 			case 36:
-				{t.kind = 74; break;}
+				{t.kind = 76; break;}
 			case 37:
-				{t.kind = 83; break;}
-			case 38:
 				{t.kind = 85; break;}
-			case 39:
-				{t.kind = 86; break;}
-			case 40:
+			case 38:
 				{t.kind = 87; break;}
-			case 41:
+			case 39:
 				{t.kind = 88; break;}
-			case 42:
+			case 40:
 				{t.kind = 89; break;}
-			case 43:
+			case 41:
 				{t.kind = 90; break;}
-			case 44:
+			case 42:
 				{t.kind = 91; break;}
-			case 45:
+			case 43:
 				{t.kind = 92; break;}
-			case 46:
+			case 44:
 				{t.kind = 93; break;}
-			case 47:
+			case 45:
+				{t.kind = 94; break;}
+			case 46:
 				{t.kind = 95; break;}
+			case 47:
+				{t.kind = 97; break;}
 			case 48:
 				if (ch == '&') {AddCh(); goto case 49;}
 				else {goto case 0;}
 			case 49:
-				{t.kind = 96; break;}
-			case 50:
-				{t.kind = 97; break;}
-			case 51:
 				{t.kind = 98; break;}
-			case 52:
+			case 50:
 				{t.kind = 99; break;}
+			case 51:
+				{t.kind = 100; break;}
+			case 52:
+				{t.kind = 101; break;}
 			case 53:
-				{t.kind = 102; break;}
-			case 54:
-				{t.kind = 103; break;}
-			case 55:
 				{t.kind = 104; break;}
-			case 56:
+			case 54:
 				{t.kind = 105; break;}
-			case 57:
+			case 55:
 				{t.kind = 106; break;}
+			case 56:
+				{t.kind = 107; break;}
+			case 57:
+				{t.kind = 108; break;}
 			case 58:
-				{t.kind = 115; break;}
-			case 59:
 				{t.kind = 117; break;}
-			case 60:
-				{t.kind = 118; break;}
-			case 61:
+			case 59:
 				{t.kind = 119; break;}
+			case 60:
+				{t.kind = 120; break;}
+			case 61:
+				{t.kind = 121; break;}
 			case 62:
 				recEnd = pos; recKind = 6;
 				if (ch == '=') {AddCh(); goto case 32;}
@@ -765,10 +767,10 @@ public class Scanner {
 				else if (ch == ':') {AddCh(); goto case 60;}
 				else {t.kind = 6; break;}
 			case 63:
-				recEnd = pos; recKind = 101;
+				recEnd = pos; recKind = 103;
 				if (ch == 'i') {AddCh(); goto case 16;}
 				else if (ch == '=') {AddCh(); goto case 39;}
-				else {t.kind = 101; break;}
+				else {t.kind = 103; break;}
 			case 64:
 				recEnd = pos; recKind = 17;
 				if (ch == '=') {AddCh(); goto case 69;}
@@ -795,17 +797,17 @@ public class Scanner {
 				if (ch == '>') {AddCh(); goto case 45;}
 				else {t.kind = 31; break;}
 			case 70:
-				recEnd = pos; recKind = 114;
+				recEnd = pos; recKind = 116;
 				if (ch == '.') {AddCh(); goto case 30;}
-				else {t.kind = 114; break;}
+				else {t.kind = 116; break;}
 			case 71:
-				recEnd = pos; recKind = 84;
+				recEnd = pos; recKind = 86;
 				if (ch == '=') {AddCh(); goto case 72;}
-				else {t.kind = 84; break;}
+				else {t.kind = 86; break;}
 			case 72:
-				recEnd = pos; recKind = 94;
+				recEnd = pos; recKind = 96;
 				if (ch == '>') {AddCh(); goto case 43;}
-				else {t.kind = 94; break;}
+				else {t.kind = 96; break;}
 
 		}
 		t.val = new String(tval, 0, tlen);
